newchan -> newbarrier

barrier/barrier.v
@@ -1,10 +1,10 @@
 From heap_lang Require Export substitution notation.
 
-Definition newchan : val := λ: "", ref '0.
+Definition newbarrier : val := λ: "", ref '0.
 Definition signal : val := λ: "x", "x" <- '1.
 Definition wait : val :=
   rec: "wait" "x" := if: !"x" = '1 then '() else "wait" "x".
 
-Instance newchan_closed : Closed newchan. Proof. solve_closed. Qed.
+Instance newbarrier_closed : Closed newbarrier. Proof. solve_closed. Qed.
 Instance signal_closed : Closed signal. Proof. solve_closed. Qed.
 Instance wait_closed : Closed wait. Proof. solve_closed. Qed.
