barrier/specification.v
@@ -12,7 +12,7 @@ Local Notation iProp := (iPropG heap_lang Σ).
 Lemma barrier_spec (heapN N : namespace) :
   heapN ⊥ N →
   ∃ recv send : loc → iProp -n> iProp,
-    (∀ P, heap_ctx heapN ⊑ {{ True }} newchan '() {{ λ v, ∃ l, v = LocV l ★ recv l P ★ send l P }}) ∧
+    (∀ P, heap_ctx heapN ⊑ {{ True }} newbarrier '() {{ λ v, ∃ l, v = LocV l ★ recv l P ★ send l P }}) ∧
     (∀ l P, {{ send l P ★ P }} signal (LocV l) {{ λ _, True }}) ∧
     (∀ l P, {{ recv l P }} wait (LocV l) {{ λ _, P }}) ∧
     (∀ l P Q, {{ recv l (P ★ Q) }} Skip {{ λ _, recv l P ★ recv l Q }}) ∧
@@ -22,7 +22,7 @@ Proof.
   exists (λ l, CofeMor (recv heapN N l)), (λ l, CofeMor (send heapN N l)).
   split_and?; simpl.
   - intros P. apply: always_intro. apply impl_intro_r.
-    rewrite -(newchan_spec heapN N P) // always_and_sep_r.
+    rewrite -(newbarrier_spec heapN N P) // always_and_sep_r.
     apply sep_mono_r, forall_intro=>l; apply wand_intro_l.
     by rewrite right_id -(exist_intro l) const_equiv // left_id.
   - intros l P. apply ht_alt. by rewrite -signal_spec right_id.
